wip: add bignum_from_bytes and bignum_to_bytes

code/experimental/rsapss/Hacl.Bignum.Convert.fst
@@ -11,97 +11,95 @@ open Lib.ByteBuffer
 open Hacl.Bignum
 
 module ST = FStar.HyperStack.ST
+module LSeq = Lib.Sequence
+module BSeq = Lib.ByteSequence
+
 module S = Spec.RSAPSS
+module SC = Hacl.Spec.Bignum.Convert
 
 
 #reset-options "--z3rlimit 50 --max_fuel 0 --max_ifuel 0"
 
 inline_for_extraction noextract
-val text_to_nat_:
-    len:size_t
-  -> input:lbuffer uint8 len
-  -> resLen:size_t{v len = 8 * v resLen}
-  -> res:lbignum resLen ->
+val bignum_from_bytes_:
+    len:size_t{8 * v len <= max_size_t}
+  -> b:lbuffer uint8 (8ul *! len)
+  -> res:lbignum len ->
   Stack unit
-  (requires fun h -> live h input /\ live h res /\ disjoint res input)
-  (ensures  fun h0 _ h1 -> modifies (loc res) h0 h1)
-
-let text_to_nat_ len input resLen res =
-  let h0 = ST.get () in
-  let inv h1 i = modifies (loc res) h0 h1 in
-  Lib.Loops.for 0ul resLen inv
-  (fun i ->
-    res.(resLen -! i -! 1ul) <- uint_from_bytes_be (sub input (8ul *! i) 8ul)
-  )
-
-
-val text_to_nat:
-    len:size_t{v len > 0}
-  -> input:lbuffer uint8 len
-  -> res:lbignum (blocks len 8ul){8 * v (blocks len 8ul) <= max_size_t} ->
-  Stack unit
-  (requires fun h -> live h input /\ live h res /\ disjoint res input)
+  (requires fun h -> live h b /\ live h res /\ disjoint res b)
   (ensures  fun h0 _ h1 -> modifies (loc res) h0 h1 /\
-    bn_v h1 res == S.os2ip #(v len) (as_seq h0 input))
+    as_seq h1 res == SC.bignum_from_bytes_ (v len) (as_seq h0 b))
 
-[@"c_inline"]
-let text_to_nat len input res = admit();
+let bignum_from_bytes_ len b res =
+  let h0 = ST.get () in
+  [@inline_let]
+  let spec h = SC.bignum_from_bytes_f (v len) (as_seq h b) in
+  fill h0 len res spec
+  (fun j -> uint_from_bytes_be (sub b ((len -! j -! 1ul) *! 8ul) 8ul))
+
+
+val bignum_from_bytes:
+    len:size_t{0 < v len /\ 8 * v (blocks len 8ul) <= max_size_t}
+  -> b:lbuffer uint8 len
+  -> res:lbignum (blocks len 8ul) ->
+  Stack unit
+  (requires fun h -> live h b /\ live h res /\ disjoint res b)
+  (ensures  fun h0 _ h1 -> modifies (loc res) h0 h1 /\
+    bn_v h1 res == S.os2ip #(v len) (as_seq h0 b))
+
+[@CInline]
+let bignum_from_bytes len b res =
+  let h0 = ST.get () in
   push_frame ();
-  let num_words = blocks len 8ul in
-  let tmpLen = 8ul *! num_words in
-  let m = len %. 8ul in
-  let ind = if m =. 0ul then 0ul else 8ul -. m in
-
+  let bnLen = blocks len 8ul in
+  let tmpLen = 8ul *! bnLen in
   let tmp = create tmpLen (u8 0) in
-  let tmpLen1 = tmpLen -. ind in
-  let tmp1 = sub tmp ind tmpLen1 in
-  copy tmp1 input;
-  text_to_nat_ tmpLen tmp num_words res;
+  update_sub tmp (tmpLen -! len) len b;
+  bignum_from_bytes_ bnLen tmp res;
+  SC.bignum_from_bytes_lemma (v len) (as_seq h0 b);
   pop_frame ()
 
 
 inline_for_extraction noextract
-val nat_to_text_:
-    len:size_t
-  -> input:lbignum len
-  -> resLen:size_t{v resLen = 8 * v len}
-  -> res:lbuffer uint8 resLen ->
+val bignum_to_bytes_:
+    len:size_t{8 * v len <= max_size_t}
+  -> b:lbignum len
+  -> res:lbuffer uint8 (8ul *! len) ->
   Stack unit
-  (requires fun h -> live h input /\ live h res /\ disjoint res input)
-  (ensures  fun h0 _ h1 -> modifies (loc res) h0 h1)
+  (requires fun h -> live h b /\ live h res /\ disjoint res b)
+  (ensures  fun h0 _ h1 -> modifies (loc res) h0 h1 /\
+    as_seq h1 res == SC.bignum_to_bytes_ (v len) (as_seq h0 b))
 
-let nat_to_text_ len input resLen res =
+let bignum_to_bytes_ len b res =
   let h0 = ST.get () in
-  let inv h1 i = modifies (loc res) h0 h1 in
-  Lib.Loops.for 0ul len inv
-  (fun i ->
-    let tmp = input.(len -. i -. 1ul) in
-    uint_to_bytes_be (sub res (8ul *. i) 8ul) tmp
-  )
+  [@ inline_let]
+  let a_spec (i:nat{i <= v len}) = unit in
+  [@ inline_let]
+  let spec (h:mem) = SC.bignum_to_bytes_f (v len) (as_seq h b) in
+  fill_blocks h0 8ul len res a_spec (fun _ _ -> ()) (fun _ -> LowStar.Buffer.loc_none) spec
+  (fun j -> uint_to_bytes_be (sub res (j *! 8ul) 8ul) b.(len -! j -! 1ul));
+  assert_norm (SC.bignum_to_bytes_ (v len) (as_seq h0 b) == norm [delta] SC.bignum_to_bytes_ (v len) (as_seq h0 b))
 
 
-val nat_to_text:
-    len:size_t{v len > 0}
-  -> input:lbignum (blocks len 8ul){8 * v (blocks len 8ul) <= max_size_t}
+val bignum_to_bytes:
+    len:size_t{0 < v len /\ 8 * v (blocks len 8ul) <= max_size_t}
+  -> b:lbignum (blocks len 8ul)
   -> res:lbuffer uint8 len ->
   Stack unit
   (requires fun h ->
-    live h input /\ live h res /\ disjoint res input /\
-    bn_v h input < pow2 (8 * v len))
+    live h b /\ live h res /\ disjoint res b /\
+    bn_v h b < pow2 (8 * v len))
   (ensures  fun h0 _ h1 -> modifies (loc res) h0 h1 /\
-    as_seq h1 res == S.i2osp #(v len) (bn_v h0 input))
+    as_seq h1 res == S.i2osp #(v len) (bn_v h0 b))
 
-[@"c_inline"]
-let nat_to_text len input res = admit();
+[@CInline]
+let bignum_to_bytes len b res =
+  let h0 = ST.get () in
   push_frame ();
-  let num_words = blocks len 8ul in
-  let tmpLen = 8ul *! num_words in
-  let m = len %. 8ul in
-  let ind = if m =. 0ul then 0ul else 8ul -. m in
-
+  let bnLen = blocks len 8ul in
+  let tmpLen = 8ul *! bnLen in
   let tmp = create tmpLen (u8 0) in
-  nat_to_text_ num_words input tmpLen tmp;
-  let tmpLen1 = tmpLen -. ind in
-  let tmp1 = sub tmp ind tmpLen1 in
-  copy res tmp1;
+  bignum_to_bytes_ bnLen b tmp;
+  copy res (sub tmp (tmpLen -! len) len);
+  SC.bignum_to_bytes_lemma (v len) (as_seq h0 b);
   pop_frame ()
